\documentclass{article}
\usepackage{amsthm}
\begin{document}
	\begin{center}
		\large{\textbf{Equations in LaTeX}}
	\end{center}
	
	\section*{Equation 1}
	$x = \frac{-b \pm \sqrt{b^2 - 4ac}}{2a}$\\
	
	$= \frac{-2 \pm \sqrt{2^2 - 4 \cdot 1 \cdot (-8)}}{2 \cdot 1}$\\
	
	$= \frac{-2 \pm \sqrt{4 + 32}}{2}$\\
	
	\section*{Equation 2}
	$\varphi^{\lambda}_{\sigma}a_{t} + \sum_{\pi \in c_{t}} 
	sgn(\pi)\varphi^{\lambda}_{\pi}$\\
	
	$= \sum_{\tau \in c_{\sigma t}} sgn(\sigma^{-1} \tau \sigma) 
	\varphi^{\lambda}_{\sigma} \varphi^{\lambda}_{\sigma^{-1} \tau \sigma}$\\
	
	$= a_{\sigma t} \varphi^{\lambda}_{\sigma}$\\
	
\end{document}